veric/Clight_assert_lemmas.v
@@ -17,9 +17,6 @@ assert_of (fun rho =>
   ⌜(glob_specs Delta) !! id = Some fs⌝ →
   (∃ b : block, ⌜Map.get (ge_of rho) id = Some b⌝ ∧ func_ptr_si (ge_of rho) E id fs (Vptr b Ptrofs.zero))).
 
-Global Instance funspec_inhabited : Inhabited (@funspec Σ).
-Proof. constructor. exact (mk_funspec ([], Tvoid) cc_default unit (fun _ _ => True) (fun _ _ => True)). Qed.
-
 Definition allp_fun_id_sigcc (Delta : tycontext) : assert :=
 assert_of (fun rho =>
 (∀ id : ident ,
